progress

src/AggregatingProgram.v
@@ -160,6 +160,11 @@ Definition is_blank (e : expr) :=
 (* Definition meta_rule_of (p : list rule) (r : bare_rule) := *)
 (*   let (concl, hyps) := r in *)
 
+Definition closure_rule (p : list rule) R (Rs : list rel) : rule :=
+  normal_rule
+    [{| clause_R := (R, meta); clause_args := [closure p (map var_expr (seq O (length Rs))); lit blank] |}]
+    (map (fun '(R', i) => {| clause_R := (R', meta); clause_args := [var_expr i; lit blank] |}) (combine Rs (seq O (length Rs)))).
+
 Fixpoint compile_Sexpr (name : nat) (out : rel) {t} (e : Sexpr (fun _ => nat) t) : nat * list rule * (list rule -> list rule) :=
   match e with
   | Var t x => (name,
@@ -167,10 +172,7 @@ Fixpoint compile_Sexpr (name : nat) (out : rel) {t} (e : Sexpr (fun _ => nat) t)
                    [{| clause_R := (out, normal); clause_args := [var_expr O] |}]
                    [{| clause_R := (x, normal); clause_args := [var_expr O] |}]],
                 fun p =>
-                  [normal_rule
-                     [{| clause_R := (out, meta); clause_args := [closure p [var_expr O]; lit blank] |}]
-                     [{| clause_R := (x, meta); clause_args := [var_expr O; lit blank] |}]
-              ])
+                  [closure_rule p out [x]])
   | bop_over_vals o x y =>
       let x' := name in
       let '(name1, p1, p1') := compile_Sexpr (S name) x' x in
@@ -205,12 +207,7 @@ Fixpoint compile_Sexpr (name : nat) (out : rel) {t} (e : Sexpr (fun _ => nat) t)
           [{| clause_R := (x', normal); clause_args := [var_expr O] |};
            {| clause_R := (y', normal); clause_args := [var_expr O] |}]
           :: p1 ++ p2,
-        fun p =>
-          normal_rule
-            [{| clause_R := (out, meta); clause_args := [closure p [var_expr O; var_expr (S O)]] |}]
-            [{| clause_R := (x', meta); clause_args := [var_expr O; lit blank] |};
-             {| clause_R := (y', meta); clause_args := [var_expr O; lit blank] |}]
-            :: p1' p ++ p2' p)
+        fun p => closure_rule p out [x'; y'] :: p1' p ++ p2' p)
   | let_in t1 t2 x y =>
       let x' := name in
       let '(name1, p1, p1') := compile_Sexpr (S name) x' x in
@@ -383,18 +380,67 @@ Ltac interp_exprs :=
 
 Definition mrs_very_sound_for (p : list rule) R :=
   forall Q S0,
+    (forall f, Q f -> f.(fact_R) <> (R, normal)) ->
     prog_impl_implication p Q {| fact_R := (R, meta); fact_args := [factset S0; blank] |} ->
     forall x,
       prog_impl_implication p Q {| fact_R := (R, normal); fact_args := [primitive x] |} <->
         S0 (R, [x]).
 
-Definition closure_rule (p : list rule) R (Rs : list unit) : rule :=
-  normal_rule
-    [{| clause_R := (R, meta); clause_args := [closure p (map var_expr (seq O (length Rs))); lit blank] |}]
-    [].
+(*i want to say that R depends only on Rs*)
+Definition depends_only_on (p : list rule) R Rs :=
+  forall Q x,
+    prog_impl_implication p Q {| fact_R := (R, normal); fact_args := [primitive x] |} ->
+    Q ({| fact_R := (R, normal); fact_args := [primitive x] |}) \/
+      prog_impl_implication p (fun f => Q f /\ In (fst f.(fact_R)) Rs) {| fact_R := (R, normal); fact_args := [primitive x] |}.
 
-Definition describes R Rs p :=
+Definition syntactically_depends_only_on (p : list rule) R Rs :=
+  Forall (fun r => In R (concl_rels r) -> incl (hyp_rels r) Rs) p.
 
+Lemma depends_only_on_mrs_very_sound_for p R Rs :
+  (*this hypothesis should be more fine-grained; we just need that R meta-facts don't allow any new conclusions from p*)
+  ~In R (flat_map hyp_rels p) ->
+  ~In R Rs ->
+  (*seems ugly to require Rs <> []..*)
+  depends_only_on p R Rs ->
+  mrs_very_sound_for p R ->
+  mrs_very_sound_for (closure_rule p R Rs :: p) R.
+Proof.
+  intros HR1 HR2 HRs Hp. intros Q S0 HQ HS0 x. split; intros Hx.
+  - assert (Hstaged : disjoint_lists [R] (flat_map hyp_rels p)).
+    { simpl. apply disjoint_lists_alt. constructor; [|constructor].
+      apply Forall_forall. intros x0 Hx0 ?. subst. auto. }
+    assert (Hloopless : disjoint_lists
+                          (flat_map concl_rels [closure_rule p R Rs])
+                          (flat_map hyp_rels [closure_rule p R Rs])).
+    { simpl. do 2 rewrite map_map. apply disjoint_lists_alt.
+      constructor; [|constructor]. rewrite app_nil_r.
+      rewrite map_ext with (g := fst).
+      2: { intros (?, ?). reflexivity. }
+      rewrite map_combine_fst.
+      - apply Forall_forall. intros ? ? ?. subst. auto.
+      - rewrite length_seq. reflexivity. }
+    rewrite cons_is_app in HS0.
+    apply staged_program in HS0; [|assumption].
+    apply loopless_program in HS0; [|assumption].
+    rewrite cons_is_app in Hx.
+    apply staged_program in Hx; [|assumption].
+    apply loopless_program in Hx; [|assumption].
+    destruct Hx as [Hx|Hx].
+    2: { clear -Hx. fwd. invert_stuff. }
+    destruct HS0 as [HS0|HS0].
+    { apply Hp in HS0. 2: assumption. apply HS0. assumption. }
+    cbv [depends_only_on] in HRs. specialize (HRs _ _ Hx).
+    destruct HRs as [HRs|HRs].
+    {
+    fwd. invert_stuff. clear Hstaged Hloopless.
+    simpl in *. invert_stuff. destruct (option_all _) eqn:E; [|discriminate]. fwd.
+    apply option_all_Forall2 in E. Search q. simpl. move HRs at bottom.
+      Search q.
+      Search option_all. subst.
+      fwd.
+
+      assumption.
+         instantiate reflexivity. apply Forall_map.
 
 Lemma compile_Sexpr_correct datalog_ctx ctx t e e_nat e' name out name' p p' :
   wf_Sexpr ctx t e e_nat ->
